Split into multiple files

src/tactic/auto/tree.lean
@@ -4,232 +4,15 @@ Released under Apache 2.0 license as described in the file LICENSE.
 Authors: Jannis Limperg
 -/
 
-import tactic.core
-
-/-!
-# `auto`, a general-purpose proof search tactic
--/
-
-/-
-TODO:
-
-- Metavariables need to be reset when we switch between branches of the search
-  tree. Currently, mvars may leak freely between branches. Maybe the best
-  solution here is to disallow proof rules from introducing new metas, except
-  for those which represent goals. auto could check this at runtime, or elide
-  the check for efficiency unless a 'debug mode' is toggled.
-- Rule indexing. Currently, we iterate through the list of rules one-by-one,
-  which is a tiny bit inefficient.
--/
-
-universes u v w
-
-/-!
-## Utility stuff
--/
-
-namespace list
-
-def find_and_remove {α} (p : α → Prop) [decidable_pred p] :
-  list α → option (α × list α)
-| [] := none
-| (a :: as) :=
-  if p a
-    then some (a, as)
-    else do
-      (x, as) ← find_and_remove as,
-      pure (x, a :: as)
-
-end list
-
-namespace native.rb_lmap
-
-open native
-
-meta def insert_list {α β} (m : rb_lmap α β) (a : α) (bs : list β) : rb_lmap α β :=
-match rb_map.find m a with
-| none := rb_map.insert m a bs
-| some bs' := rb_map.insert m a (bs ++ bs')
-end
-
-end native.rb_lmap
-
-namespace format
-
-open tactic
-
-meta def unlines : list format → format :=
-intercalate line
-
-meta def nested (n : ℕ) (f : format) : format :=
-if f.is_nil
-  then nil
-  else nest n $ format.line ++ f
-
-meta def of_goal (e : expr) : tactic format :=
-if e.is_mvar
-  then with_local_goals' [e] $ read >>= pp
-  else pp e
-
-end format
+import tactic.auto.rule
+import tactic.auto.util
 
 namespace tactic
 namespace auto
 
-open expr
 open native
 
-/-!
-## Mock implementation of prio queues
--/
-
-structure priority_queue (α : Type u) (lt : α → α → bool) :=
-(queue : list α)
-
-namespace priority_queue
-
-variables {α : Type u} {lt : α → α → bool}
-
-def empty : priority_queue α lt :=
-⟨[]⟩
-
-def singleton (a : α) : priority_queue α lt :=
-⟨[a]⟩
-
-def from_list (as : list α) : priority_queue α lt :=
-⟨list.qsort lt as⟩
-
-def is_empty (q : priority_queue α lt) : bool :=
-q.queue.empty
-
-def insert (a : α) (q : priority_queue α lt) : priority_queue α lt :=
-⟨list.qsort lt $ a :: q.queue⟩
-
-def insert_list (as : list α) (q : priority_queue α lt) : priority_queue α lt :=
-⟨list.qsort lt $ as ++ q.queue⟩
-
-def pop_min (q : priority_queue α lt) : option (α × priority_queue α lt) :=
-match q.queue with
-| [] := none
-| (a :: as) := some (a, ⟨as⟩)
-end
-
-def filter (p : α → Prop) [decidable_pred p] (q : priority_queue α lt) :
-  priority_queue α lt :=
-⟨q.queue.filter p⟩
-
-def to_list (q : priority_queue α lt) : list α :=
-q.queue
-
-end priority_queue
-
-/-!
-## Rules
--/
-
-meta structure rule :=
-(penalty : ℕ)
-(tac : tactic unit)
-(description : format)
-
-namespace rule
-
-protected meta def to_fmt (r : rule) : format :=
-format.sbracket (_root_.to_fmt r.penalty) ++ format.space ++ r.description
-
-meta instance : has_to_format rule :=
-⟨rule.to_fmt⟩
-
-meta def make_apply (e : expr) (penalty : ℕ) : tactic rule :=
-pure
-  { tac := apply e >> skip,
-    penalty := penalty,
-    description := format! "apply {e}" }
-
-meta def make_const_apply (n : name) (penalty : ℕ) : tactic rule := do
-  n ← resolve_constant n,
-  pure
-    { tac := mk_const n >>= apply >> skip,
-      penalty := penalty,
-      description := format! "apply {n}" }
-
-protected meta def lt (r s : rule) : bool :=
-r.penalty < s.penalty
-
-end rule
-
-/-!
-## Rule Set
--/
-
-meta structure rule_set :=
-(rules : list rule)
-
-namespace rule_set
-
-protected meta def to_fmt (rs : rule_set) : format :=
-format.unlines $ rs.rules.map rule.to_fmt
-
-meta instance : has_to_format rule_set :=
-⟨rule_set.to_fmt⟩
-
-meta def empty : rule_set :=
-⟨[]⟩
-
-meta def add (r : rule) (rs : rule_set) : rule_set :=
-⟨r :: rs.rules⟩
-
-meta def mfold {α} (rs : rule_set) (init : α) (f : α → rule → tactic α) : tactic α :=
-rs.rules.mfoldl f init
-
-meta def first {α} (rs : rule_set) (f : rule → tactic α) : tactic α :=
-rs.rules.mfirst f
-
-meta def merge (rs₁ rs₂ : rule_set) : rule_set :=
-⟨rs₁.rules ++ rs₂.rules⟩
-
-meta def from_list (rs : list rule) : rule_set :=
-⟨rs⟩
-
-meta def applicable_rules (rs : rule_set) : tactic (list rule) :=
-pure rs.rules
-
-end rule_set
-
-/-!
-## Attribute
--/
-
-namespace attr
-
-open lean.parser
-
-@[user_attribute]
-meta def attr : user_attribute name_set ℕ :=
-{ name := `auto,
-  descr := "Registers a definition as a rule for the auto tactic.",
-  cache_cfg := {
-    mk_cache := pure ∘ name_set.of_list,
-    dependencies := [] },
-  parser := small_nat }
-
-meta def declaration_to_rule (decl : name) (penalty : ℕ) : tactic rule :=
-rule.make_const_apply decl penalty
-
-meta def declarations_to_rule_set (decls : name_set) : tactic rule_set :=
-rule_set.from_list <$> decls.to_list.mmap (λ decl, do {
-  penalty ← attr.get_param decl,
-  declaration_to_rule decl penalty
-})
-
-meta def registered_rule_set : tactic rule_set :=
-attr.get_cache >>= declarations_to_rule_set
-
-end attr
-
-/-!
-## Search
--/
+/-! ## Node IDs -/
 
 @[derive decidable_eq]
 meta structure node_id :=
@@ -264,6 +47,8 @@ meta instance : has_to_format node_id :=
 
 end node_id
 
+/-! ## Rule Application IDs -/
+
 @[derive decidable_eq]
 meta structure rapp_id :=
 (to_nat : ℕ)
@@ -296,6 +81,8 @@ meta instance : has_to_format rapp_id :=
 ⟨rapp_id.to_fmt⟩
 
 end rapp_id
+
+/-! ## Nodes -/
 
 meta structure node :=
 (parent : option rapp_id)
@@ -334,6 +121,8 @@ meta def is_unknown (n : node) : bool :=
 ¬ n.is_proven ∧ ¬ n.is_unprovable
 
 end node
+
+/-! ## Rule Applications -/
 
 /- Rule application. -/
 meta structure rapp :=
@@ -609,213 +398,5 @@ meta instance : has_to_tactic_format tree :=
 
 end tree
 
-meta structure unexpanded_rapp :=
-(parent : node_id)
-(rule : rule)
-
-namespace unexpanded_rapp
-
-protected meta def lt (n m : unexpanded_rapp) : bool :=
-n.rule.penalty < m.rule.penalty
-
-protected meta def to_fmt (n : unexpanded_rapp) : format :=
-"for node " ++ n.parent.to_fmt ++ ": " ++ n.rule.to_fmt
-
-meta instance : has_to_format unexpanded_rapp :=
-⟨unexpanded_rapp.to_fmt⟩
-
-end unexpanded_rapp
-
-meta structure state :=
-(search_tree : tree)
-(unexpanded_rapps : priority_queue unexpanded_rapp unexpanded_rapp.lt)
-
-namespace state
-
-protected meta def to_tactic_format (s : state) : tactic format := do
-  t ← pp s.search_tree,
-  let unexpanded :=
-    format.unlines $ s.unexpanded_rapps.to_list.map unexpanded_rapp.to_fmt,
-  pure $ format.join
-    [ "search tree:"
-    , format.nested 2 t
-    , format.line
-    , "unexpanded nodes:"
-    , format.nested 2 unexpanded
-    ]
-
-meta instance : has_to_tactic_format state :=
-⟨state.to_tactic_format⟩
-
-meta def empty : state :=
-{ search_tree := tree.empty,
-  unexpanded_rapps := priority_queue.empty }
-
-end state
-
-meta def select_rules (rs : rule_set) (id : node_id) (goal : expr) :
-  tactic (list unexpanded_rapp) := do
-  rules ← with_local_goals' [goal] $ rs.applicable_rules,
-  pure $ rules.map $ λ r, { parent := id, rule := r }
-
-meta def add_node (rs : rule_set) (s : state) (goal : expr)
-  (parent : option rapp_id) : tactic (node_id × state) := do
-  let n : node :=
-    { parent := parent,
-      goal := goal,
-      num_rules_todo := 0,
-      rapps := [],
-      failed_rapps := [],
-      is_proven := ff,
-      is_unprovable := ff,
-      is_irrelevant := ff },
-  let (id, t) := s.search_tree.insert_node n,
-  unexpanded_rapps ← select_rules rs id goal,
-  let t := t.modify_node id $ λ n,
-    { num_rules_todo := unexpanded_rapps.length, ..n },
-  let s : state :=
-    { unexpanded_rapps := s.unexpanded_rapps.insert_list unexpanded_rapps,
-      search_tree := t },
-  pure (id, s)
-
-meta def add_nodes (rs : rule_set) (s : state) (goals : list expr)
-  (parent : rapp_id) : tactic (list node_id × state) :=
-goals.mfoldl
-  (λ ⟨ids, s⟩ goal, do
-    (id, s) ← add_node rs s goal parent,
-    pure (id :: ids, s))
-  ([], s)
-
-meta def initial_state (rs : rule_set) : tactic state := do
-  goal ← get_goal,
-  prod.snd <$> add_node rs state.empty goal none
-
-meta def run_rule (goal : expr) (r : rule) : tactic (option (expr × list expr)) :=
-with_local_goals' [goal] $ do
-  tgt ← target,
-  goal' ← mk_meta_var tgt,
-  set_goals [goal'],
-  try_core $ do
-    r.tac,
-    subgoals ← get_goals,
-    pure (goal', subgoals)
-
-meta def expand_rapp (rs : rule_set) (s : state) (n : unexpanded_rapp) :
-  tactic state := do
-  let parent_id := n.parent,
-  let rule := n.rule,
-  let t := s.search_tree.modify_node parent_id $ λ parent,
-    { num_rules_todo := parent.num_rules_todo - 1, ..parent },
-  rule_result ← do {
-    parent ← t.get_node' parent_id "auto/expand/rapp: internal error: ",
-    run_rule parent.goal rule },
-  s ← match rule_result with
-      | some (prf, []) := do
-          -- Rule succeeded and did not generate subgoals, meaning the parent
-          -- node is proven.
-          -- 1. Record the rule application.
-          let r : rapp :=
-            { applied_rule := rule,
-              proof := prf,
-              subgoals := [],
-              parent := parent_id,
-              is_proven := tt,
-              is_unprovable := ff,
-              is_irrelevant := ff },
-          let (rid, t) := t.insert_rapp r,
-          -- 2. Mark parent node, and potentially ancestors, as proven.
-          let t := t.set_node_proven parent_id,
-          pure { search_tree := t, ..s }
-      | some (prf, subgoals) := do
-          -- Rule succeeded and generated subgoals.
-          -- 1. Record the rule application.
-          let r : rapp :=
-            { applied_rule := rule,
-              proof := prf,
-              subgoals := [],
-              parent := parent_id,
-              is_proven := ff,
-              is_unprovable := ff,
-              is_irrelevant := ff },
-          let (rid, t) := t.insert_rapp r,
-          let s := { search_tree := t, ..s },
-          -- 2. Record the subgoals.
-          (_, s) ← add_nodes rs s subgoals rid,
-          -- 2. Add an active rule application with the generated subgoals.
-          pure s
-      | none := do
-          -- Rule did not succeed.
-          -- 1. Record rule failure.
-          let t := t.modify_node parent_id $ λ parent,
-            { failed_rapps := rule :: parent.failed_rapps, ..parent },
-          -- 2. Potentially mark parent node (and ancestors) as unprovable.
-          let t := t.set_node_unprovable parent_id,
-          pure { search_tree := t, ..s }
-      end,
-  trace "---------------------------------------------------------------------",
-  trace s,
-  pure s
-
-meta def expand (rs : rule_set) (s : state) : tactic (option state) := do
-  trace "=====================================================================",
-  trace s,
-  some (to_expand, unexpanded_rapps) ← pure s.unexpanded_rapps.pop_min
-    | pure none,
-  trace "---------------------------------------------------------------------",
-  trace! "expanding for node {to_expand.parent}: {to_expand.rule}",
-  let s := { unexpanded_rapps := unexpanded_rapps, ..s },
-  parent ← s.search_tree.get_node' to_expand.parent
-    "auto/expand: internal error: ",
-  if parent.is_proven ∨ parent.is_unprovable ∨ parent.is_irrelevant
-    then pure (some s)
-    else some <$> expand_rapp rs s to_expand
-
-meta def finish_if_proven (s : state) : tactic bool := do
-  tt ← pure $ s.search_tree.root_node_is_proven
-    | pure ff,
-  s.search_tree.link_proofs,
-  prf ← s.search_tree.extract_proof,
-  exact prf,
-  pure tt
-
-private meta def search_loop (rs : rule_set) : state → tactic unit := λ s, do
-  ff ← pure $ s.search_tree.root_node_is_unprovable
-    | fail "auto: failed to prove the goal",
-  done ← finish_if_proven s,
-  when ¬ done $ do
-    (some s) ← expand rs s
-      | fail "auto: internal error: no more rules to apply but root node is not marked as unprovable",
-    search_loop s
-
-meta def search (rs : rule_set) : tactic unit :=
-initial_state rs >>= search_loop rs
-
-meta def auto : tactic unit :=
-attr.registered_rule_set >>= search
-
 end auto
 end tactic
-
-/-!
-## Tests
--/
-
-open tactic.auto
-
-inductive Even : ℕ → Prop
-| zero : Even 0
-| plus_two {n} : Even n → Even (n + 2)
-
-inductive Odd : ℕ → Prop
-| one : Odd 1
-| plus_two {n} : Odd n → Odd (n + 2)
-
-inductive EvenOrOdd : ℕ → Prop
-| even {n} : Even n → EvenOrOdd n
-| odd {n} : Odd n → EvenOrOdd n
-
-attribute [auto 10] EvenOrOdd.odd EvenOrOdd.even
-attribute [auto  1] Even.zero Even.plus_two
-attribute [auto  0] Odd.one Odd.plus_two
-
-example : EvenOrOdd 3 := by auto
