src/tactic/auto/attribute.lean
@@ -1,0 +1,39 @@
+/-
+Copyright (c) 2021 Jannis Limperg. All rights reserved.
+Released under Apache 2.0 license as described in the file LICENSE.
+Authors: Jannis Limperg
+-/
+
+import tactic.auto.rule
+
+namespace tactic
+namespace auto
+
+open lean.parser
+
+@[user_attribute]
+meta def attr : user_attribute name_set ℕ :=
+{ name := `auto,
+  descr := "Registers a definition as a rule for the auto tactic.",
+  cache_cfg := {
+    mk_cache := pure ∘ name_set.of_list,
+    dependencies := [] },
+  parser := small_nat }
+
+namespace attr
+
+meta def declaration_to_rule (decl : name) (penalty : ℕ) : tactic rule :=
+rule.make_const_apply decl penalty
+
+meta def declarations_to_rule_set (decls : name_set) : tactic rule_set :=
+rule_set.from_list <$> decls.to_list.mmap (λ decl, do {
+  penalty ← attr.get_param decl,
+  declaration_to_rule decl penalty
+})
+
+meta def registered_rule_set : tactic rule_set :=
+attr.get_cache >>= declarations_to_rule_set
+
+end attr
+end auto
+end tactic
