src/tactic/auto/default.lean
@@ -1,0 +1,250 @@
+/-
+Copyright (c) 2021 Jannis Limperg. All rights reserved.
+Released under Apache 2.0 license as described in the file LICENSE.
+Authors: Jannis Limperg
+-/
+
+import tactic.auto.attribute
+import tactic.auto.priority_queue
+import tactic.auto.tree
+
+/-!
+# `auto`, a general-purpose proof search tactic
+-/
+
+/-
+TODO:
+
+- Metavariables need to be reset when we switch between branches of the search
+  tree. Currently, mvars may leak freely between branches. Maybe the best
+  solution here is to disallow proof rules from introducing new metas, except
+  for those which represent goals. auto could check this at runtime, or elide
+  the check for efficiency unless a 'debug mode' is toggled.
+- Rule indexing. Currently, we iterate through the list of rules one-by-one,
+  which is a tiny bit inefficient.
+-/
+
+namespace tactic
+namespace auto
+
+/-! ## Unexpanded Rule Applications -/
+
+meta structure unexpanded_rapp :=
+(parent : node_id)
+(rule : rule)
+
+namespace unexpanded_rapp
+
+protected meta def lt (n m : unexpanded_rapp) : bool :=
+n.rule.penalty < m.rule.penalty
+
+protected meta def to_fmt (n : unexpanded_rapp) : format :=
+"for node " ++ n.parent.to_fmt ++ ": " ++ n.rule.to_fmt
+
+meta instance : has_to_format unexpanded_rapp :=
+⟨unexpanded_rapp.to_fmt⟩
+
+end unexpanded_rapp
+
+/-! ## Search State -/
+
+meta structure state :=
+(search_tree : tree)
+(unexpanded_rapps : priority_queue unexpanded_rapp unexpanded_rapp.lt)
+
+namespace state
+
+protected meta def to_tactic_format (s : state) : tactic format := do
+  t ← pp s.search_tree,
+  let unexpanded :=
+    format.unlines $ s.unexpanded_rapps.to_list.map unexpanded_rapp.to_fmt,
+  pure $ format.join
+    [ "search tree:"
+    , format.nested 2 t
+    , format.line
+    , "unexpanded nodes:"
+    , format.nested 2 unexpanded
+    ]
+
+meta instance : has_to_tactic_format state :=
+⟨state.to_tactic_format⟩
+
+meta def empty : state :=
+{ search_tree := tree.empty,
+  unexpanded_rapps := priority_queue.empty }
+
+end state
+
+/-! ## Best-First Search -/
+
+meta def select_rules (rs : rule_set) (id : node_id) (goal : expr) :
+  tactic (list unexpanded_rapp) := do
+  rules ← with_local_goals' [goal] $ rs.applicable_rules,
+  pure $ rules.map $ λ r, { parent := id, rule := r }
+
+meta def add_node (rs : rule_set) (s : state) (goal : expr)
+  (parent : option rapp_id) : tactic (node_id × state) := do
+  let n : node :=
+    { parent := parent,
+      goal := goal,
+      num_rules_todo := 0,
+      rapps := [],
+      failed_rapps := [],
+      is_proven := ff,
+      is_unprovable := ff,
+      is_irrelevant := ff },
+  let (id, t) := s.search_tree.insert_node n,
+  unexpanded_rapps ← select_rules rs id goal,
+  let t := t.modify_node id $ λ n,
+    { num_rules_todo := unexpanded_rapps.length, ..n },
+  let s : state :=
+    { unexpanded_rapps := s.unexpanded_rapps.insert_list unexpanded_rapps,
+      search_tree := t },
+  pure (id, s)
+
+meta def add_nodes (rs : rule_set) (s : state) (goals : list expr)
+  (parent : rapp_id) : tactic (list node_id × state) :=
+goals.mfoldl
+  (λ ⟨ids, s⟩ goal, do
+    (id, s) ← add_node rs s goal parent,
+    pure (id :: ids, s))
+  ([], s)
+
+meta def initial_state (rs : rule_set) : tactic state := do
+  goal ← get_goal,
+  prod.snd <$> add_node rs state.empty goal none
+
+meta def run_rule (goal : expr) (r : rule) : tactic (option (expr × list expr)) :=
+with_local_goals' [goal] $ do
+  tgt ← target,
+  goal' ← mk_meta_var tgt,
+  set_goals [goal'],
+  try_core $ do
+    r.tac,
+    subgoals ← get_goals,
+    pure (goal', subgoals)
+
+meta def expand_rapp (rs : rule_set) (s : state) (n : unexpanded_rapp) :
+  tactic state := do
+  let parent_id := n.parent,
+  let rule := n.rule,
+  let t := s.search_tree.modify_node parent_id $ λ parent,
+    { num_rules_todo := parent.num_rules_todo - 1, ..parent },
+  rule_result ← do {
+    parent ← t.get_node' parent_id "auto/expand/rapp: internal error: ",
+    run_rule parent.goal rule },
+  s ← match rule_result with
+      | some (prf, []) := do
+          -- Rule succeeded and did not generate subgoals, meaning the parent
+          -- node is proven.
+          -- 1. Record the rule application.
+          let r : rapp :=
+            { applied_rule := rule,
+              proof := prf,
+              subgoals := [],
+              parent := parent_id,
+              is_proven := tt,
+              is_unprovable := ff,
+              is_irrelevant := ff },
+          let (rid, t) := t.insert_rapp r,
+          -- 2. Mark parent node, and potentially ancestors, as proven.
+          let t := t.set_node_proven parent_id,
+          pure { search_tree := t, ..s }
+      | some (prf, subgoals) := do
+          -- Rule succeeded and generated subgoals.
+          -- 1. Record the rule application.
+          let r : rapp :=
+            { applied_rule := rule,
+              proof := prf,
+              subgoals := [],
+              parent := parent_id,
+              is_proven := ff,
+              is_unprovable := ff,
+              is_irrelevant := ff },
+          let (rid, t) := t.insert_rapp r,
+          let s := { search_tree := t, ..s },
+          -- 2. Record the subgoals.
+          (_, s) ← add_nodes rs s subgoals rid,
+          -- 2. Add an active rule application with the generated subgoals.
+          pure s
+      | none := do
+          -- Rule did not succeed.
+          -- 1. Record rule failure.
+          let t := t.modify_node parent_id $ λ parent,
+            { failed_rapps := rule :: parent.failed_rapps, ..parent },
+          -- 2. Potentially mark parent node (and ancestors) as unprovable.
+          let t := t.set_node_unprovable parent_id,
+          pure { search_tree := t, ..s }
+      end,
+  trace "---------------------------------------------------------------------",
+  trace s,
+  pure s
+
+meta def expand (rs : rule_set) (s : state) : tactic (option state) := do
+  trace "=====================================================================",
+  trace s,
+  some (to_expand, unexpanded_rapps) ← pure s.unexpanded_rapps.pop_min
+    | pure none,
+  trace "---------------------------------------------------------------------",
+  trace! "expanding for node {to_expand.parent}: {to_expand.rule}",
+  let s := { unexpanded_rapps := unexpanded_rapps, ..s },
+  parent ← s.search_tree.get_node' to_expand.parent
+    "auto/expand: internal error: ",
+  if parent.is_proven ∨ parent.is_unprovable ∨ parent.is_irrelevant
+    then pure (some s)
+    else some <$> expand_rapp rs s to_expand
+
+meta def finish_if_proven (s : state) : tactic bool := do
+  tt ← pure $ s.search_tree.root_node_is_proven
+    | pure ff,
+  s.search_tree.link_proofs,
+  prf ← s.search_tree.extract_proof,
+  exact prf,
+  pure tt
+
+private meta def search_loop (rs : rule_set) : state → tactic unit := λ s, do
+  ff ← pure $ s.search_tree.root_node_is_unprovable
+    | fail "auto: failed to prove the goal",
+  done ← finish_if_proven s,
+  when ¬ done $ do
+    (some s) ← expand rs s
+      | fail "auto: internal error: no more rules to apply but root node is not marked as unprovable",
+    search_loop s
+
+meta def search (rs : rule_set) : tactic unit :=
+initial_state rs >>= search_loop rs
+
+meta def auto : tactic unit :=
+attr.registered_rule_set >>= search
+
+end auto
+
+meta def auto : tactic unit :=
+tactic.auto.auto
+
+meta def interactive.auto : tactic unit :=
+tactic.auto.auto
+
+end tactic
+
+/-!
+## Tests
+-/
+
+inductive Even : ℕ → Prop
+| zero : Even 0
+| plus_two {n} : Even n → Even (n + 2)
+
+inductive Odd : ℕ → Prop
+| one : Odd 1
+| plus_two {n} : Odd n → Odd (n + 2)
+
+inductive EvenOrOdd : ℕ → Prop
+| even {n} : Even n → EvenOrOdd n
+| odd {n} : Odd n → EvenOrOdd n
+
+attribute [auto 10] EvenOrOdd.odd EvenOrOdd.even
+attribute [auto  1] Even.zero Even.plus_two
+attribute [auto  0] Odd.one Odd.plus_two
+
+example : EvenOrOdd 3 := by auto
