src/tactic/auto/priority_queue.lean
@@ -1,0 +1,45 @@
+/-
+Copyright (c) 2021 Jannis Limperg. All rights reserved.
+Released under Apache 2.0 license as described in the file LICENSE.
+Authors: Jannis Limperg
+-/
+
+structure priority_queue (α : Type*) (lt : α → α → bool) :=
+(queue : list α)
+
+namespace priority_queue
+
+variables {α : Type*} {lt : α → α → bool}
+
+def empty : priority_queue α lt :=
+⟨[]⟩
+
+def singleton (a : α) : priority_queue α lt :=
+⟨[a]⟩
+
+def from_list (as : list α) : priority_queue α lt :=
+⟨list.qsort lt as⟩
+
+def is_empty (q : priority_queue α lt) : bool :=
+q.queue.empty
+
+def insert (a : α) (q : priority_queue α lt) : priority_queue α lt :=
+⟨list.qsort lt $ a :: q.queue⟩
+
+def insert_list (as : list α) (q : priority_queue α lt) : priority_queue α lt :=
+⟨list.qsort lt $ as ++ q.queue⟩
+
+def pop_min (q : priority_queue α lt) : option (α × priority_queue α lt) :=
+match q.queue with
+| [] := none
+| (a :: as) := some (a, ⟨as⟩)
+end
+
+def filter (p : α → Prop) [decidable_pred p] (q : priority_queue α lt) :
+  priority_queue α lt :=
+⟨q.queue.filter p⟩
+
+def to_list (q : priority_queue α lt) : list α :=
+q.queue
+
+end priority_queue
