src/tactic/auto/rule.lean
@@ -1,0 +1,86 @@
+/-
+Copyright (c) 2021 Jannis Limperg. All rights reserved.
+Released under Apache 2.0 license as described in the file LICENSE.
+Authors: Jannis Limperg
+-/
+
+import tactic.auto.util
+
+/-!
+## Rules
+-/
+
+namespace tactic
+namespace auto
+
+meta structure rule :=
+(penalty : ℕ)
+(tac : tactic unit)
+(description : format)
+
+namespace rule
+
+protected meta def to_fmt (r : rule) : format :=
+format.sbracket (_root_.to_fmt r.penalty) ++ format.space ++ r.description
+
+meta instance : has_to_format rule :=
+⟨rule.to_fmt⟩
+
+meta def make_apply (e : expr) (penalty : ℕ) : tactic rule :=
+pure
+  { tac := apply e >> skip,
+    penalty := penalty,
+    description := format! "apply {e}" }
+
+meta def make_const_apply (n : name) (penalty : ℕ) : tactic rule := do
+  n ← resolve_constant n,
+  pure
+    { tac := mk_const n >>= apply >> skip,
+      penalty := penalty,
+      description := format! "apply {n}" }
+
+protected meta def lt (r s : rule) : bool :=
+r.penalty < s.penalty
+
+end rule
+
+/-!
+## Rule Set
+-/
+
+meta structure rule_set :=
+(rules : list rule)
+
+namespace rule_set
+
+protected meta def to_fmt (rs : rule_set) : format :=
+format.unlines $ rs.rules.map rule.to_fmt
+
+meta instance : has_to_format rule_set :=
+⟨rule_set.to_fmt⟩
+
+meta def empty : rule_set :=
+⟨[]⟩
+
+meta def add (r : rule) (rs : rule_set) : rule_set :=
+⟨r :: rs.rules⟩
+
+meta def mfold {α} (rs : rule_set) (init : α) (f : α → rule → tactic α) : tactic α :=
+rs.rules.mfoldl f init
+
+meta def first {α} (rs : rule_set) (f : rule → tactic α) : tactic α :=
+rs.rules.mfirst f
+
+meta def merge (rs₁ rs₂ : rule_set) : rule_set :=
+⟨rs₁.rules ++ rs₂.rules⟩
+
+meta def from_list (rs : list rule) : rule_set :=
+⟨rs⟩
+
+meta def applicable_rules (rs : rule_set) : tactic (list rule) :=
+pure rs.rules
+
+end rule_set
+
+end auto
+end tactic
