src/tactic/auto/util.lean
@@ -1,0 +1,52 @@
+/-
+Copyright (c) 2021 Jannis Limperg. All rights reserved.
+Released under Apache 2.0 license as described in the file LICENSE.
+Authors: Jannis Limperg
+-/
+
+import tactic.core
+
+namespace list
+
+def find_and_remove {α} (p : α → Prop) [decidable_pred p] :
+  list α → option (α × list α)
+| [] := none
+| (a :: as) :=
+  if p a
+    then some (a, as)
+    else do
+      (x, as) ← find_and_remove as,
+      pure (x, a :: as)
+
+end list
+
+namespace native.rb_lmap
+
+open native
+
+meta def insert_list {α β} (m : rb_lmap α β) (a : α) (bs : list β) : rb_lmap α β :=
+match rb_map.find m a with
+| none := rb_map.insert m a bs
+| some bs' := rb_map.insert m a (bs ++ bs')
+end
+
+end native.rb_lmap
+
+namespace format
+
+open tactic
+
+meta def unlines : list format → format :=
+intercalate line
+
+meta def nested (n : ℕ) (f : format) : format :=
+if f.is_nil
+  then nil
+  else nest n $ format.line ++ f
+
+meta def of_goal (e : expr) : tactic format :=
+if e.is_mvar
+  then with_local_goals' [e] $ read >>= pp
+  else pp e
+
+end format
